{
 "cells": [
  {
   "cell_type": "markdown",
   "id": "53ba3460",
   "metadata": {},
   "source": [
    "Your explanation covers many fundamental ideas, but there are several points where clarity, accuracy, and the step-by-step process can be improved. Let me address your concerns and clarify key parts of the derivation.\n",
    "\n",
    "---\n",
    "\n",
    "### Revisiting Derivatives of the Cost Function\n",
    "Let’s revisit the derivatives of the Mean Squared Error (MSE) step by step for both \\( m \\) and \\( c \\).\n",
    "\n",
    "The cost function \\( J \\) (Mean Squared Error) is defined as:\n",
    "\n",
    "\\[\n",
    "J = \\frac{1}{n} \\sum_{i=1}^n \\left( y_i - \\hat{y}_i \\right)^2\n",
    "\\]\n",
    "\n",
    "Where:\n",
    "- \\( y_i \\) = actual values\n",
    "- \\( \\hat{y}_i \\) = predicted values = \\( m \\cdot x_i + c \\)\n",
    "- \\( n \\) = number of data points\n",
    "\n",
    "#### Step 1: Partial Derivative of \\( J \\) with Respect to \\( m \\)\n",
    "To minimize \\( J \\), we calculate its derivative with respect to \\( m \\). Substitute \\( \\hat{y}_i = mx_i + c \\) into \\( J \\):\n",
    "\n",
    "\\[\n",
    "J = \\frac{1}{n} \\sum_{i=1}^n \\left( y_i - (m x_i + c) \\right)^2\n",
    "\\]\n",
    "\n",
    "Let’s take the derivative \\( \\frac{\\partial J}{\\partial m} \\):\n",
    "\n",
    "1. Expand the squared term:\n",
    "   \\[\n",
    "   \\frac{\\partial J}{\\partial m} = \\frac{\\partial}{\\partial m} \\left[ \\frac{1}{n} \\sum_{i=1}^n \\left( y_i - m x_i - c \\right)^2 \\right]\n",
    "   \\]\n",
    "\n",
    "2. Move the constant \\( \\frac{1}{n} \\) outside:\n",
    "   \\[\n",
    "   \\frac{\\partial J}{\\partial m} = \\frac{1}{n} \\sum_{i=1}^n \\frac{\\partial}{\\partial m} \\left( y_i - m x_i - c \\right)^2\n",
    "   \\]\n",
    "\n",
    "3. Apply the chain rule:\n",
    "   The derivative of \\( (y_i - m x_i - c)^2 \\) is:\n",
    "   \\[\n",
    "   2 \\cdot (y_i - m x_i - c) \\cdot \\frac{\\partial}{\\partial m} \\left( y_i - m x_i - c \\right)\n",
    "   \\]\n",
    "\n",
    "4. Since \\( y_i \\) and \\( c \\) are constants with respect to \\( m \\), their derivatives are 0. The derivative of \\( -m x_i \\) with respect to \\( m \\) is \\( -x_i \\):\n",
    "   \\[\n",
    "   \\frac{\\partial J}{\\partial m} = \\frac{1}{n} \\sum_{i=1}^n 2 \\cdot (y_i - m x_i - c) \\cdot (-x_i)\n",
    "   \\]\n",
    "\n",
    "5. Simplify:\n",
    "   \\[\n",
    "   \\frac{\\partial J}{\\partial m} = -\\frac{2}{n} \\sum_{i=1}^n x_i \\cdot (y_i - m x_i - c)\n",
    "   \\]\n",
    "\n",
    "---\n",
    "\n",
    "#### Step 2: Partial Derivative of \\( J \\) with Respect to \\( c \\)\n",
    "Similarly, take the derivative of \\( J \\) with respect to \\( c \\):\n",
    "\n",
    "\\[\n",
    "\\frac{\\partial J}{\\partial c} = \\frac{\\partial}{\\partial c} \\left[ \\frac{1}{n} \\sum_{i=1}^n \\left( y_i - m x_i - c \\right)^2 \\right]\n",
    "\\]\n",
    "\n",
    "1. Move the constant \\( \\frac{1}{n} \\) outside:\n",
    "   \\[\n",
    "   \\frac{\\partial J}{\\partial c} = \\frac{1}{n} \\sum_{i=1}^n \\frac{\\partial}{\\partial c} \\left( y_i - m x_i - c \\right)^2\n",
    "   \\]\n",
    "\n",
    "2. Apply the chain rule:\n",
    "   \\[\n",
    "   \\frac{\\partial J}{\\partial c} = \\frac{1}{n} \\sum_{i=1}^n 2 \\cdot (y_i - m x_i - c) \\cdot \\frac{\\partial}{\\partial c} \\left( y_i - m x_i - c \\right)\n",
    "   \\]\n",
    "\n",
    "3. The derivative of \\( y_i - m x_i - c \\) with respect to \\( c \\) is \\( -1 \\):\n",
    "   \\[\n",
    "   \\frac{\\partial J}{\\partial c} = -\\frac{2}{n} \\sum_{i=1}^n (y_i - m x_i - c)\n",
    "   \\]\n",
    "\n",
    "---\n",
    "\n",
    "### Substituting Values\n",
    "Now that we have the gradients:\n",
    "- \\( \\frac{\\partial J}{\\partial m} = -\\frac{2}{n} \\sum_{i=1}^n x_i \\cdot (y_i - m x_i - c) \\)\n",
    "- \\( \\frac{\\partial J}{\\partial c} = -\\frac{2}{n} \\sum_{i=1}^n (y_i - m x_i - c) \\)\n",
    "\n",
    "We substitute:\n",
    "- \\( x = [1, 2, 3, 4] \\)\n",
    "- \\( y = [2, 6, 7, 12] \\)\n",
    "- \\( m = 0 \\), \\( c = 0 \\)\n",
    "\n",
    "For \\( \\frac{\\partial J}{\\partial m} \\):\n",
    "\\[\n",
    "\\frac{\\partial J}{\\partial m} = -\\frac{2}{4} \\left[ 1 \\cdot (2 - 0 \\cdot 1 - 0) + 2 \\cdot (6 - 0 \\cdot 2 - 0) + 3 \\cdot (7 - 0 \\cdot 3 - 0) + 4 \\cdot (12 - 0 \\cdot 4 - 0) \\right]\n",
    "\\]\n",
    "\\[\n",
    "= -\\frac{2}{4} (1 \\cdot 2 + 2 \\cdot 6 + 3 \\cdot 7 + 4 \\cdot 12)\n",
    "\\]\n",
    "\\[\n",
    "= -\\frac{2}{4} (2 + 12 + 21 + 48)\n",
    "\\]\n",
    "\\[\n",
    "= -\\frac{2}{4} \\cdot 83 = -41.5\n",
    "\\]\n",
    "\n",
    "For \\( \\frac{\\partial J}{\\partial c} \\):\n",
    "\\[\n",
    "\\frac{\\partial J}{\\partial c} = -\\frac{2}{4} \\left[ (2 - 0 \\cdot 1 - 0) + (6 - 0 \\cdot 2 - 0) + (7 - 0 \\cdot 3 - 0) + (12 - 0 \\cdot 4 - 0) \\right]\n",
    "\\]\n",
    "\\[\n",
    "= -\\frac{2}{4} (2 + 6 + 7 + 12)\n",
    "\\]\n",
    "\\[\n",
    "= -\\frac{2}{4} \\cdot 27 = -13.5\n",
    "\\]\n",
    "\n",
    "---\n",
    "\n",
    "### Updating \\( m \\) and \\( c \\)\n",
    "Using the gradient descent formulas:\n",
    "\\[\n",
    "m = m - \\alpha \\cdot \\frac{\\partial J}{\\partial m}\n",
    "\\]\n",
    "\\[\n",
    "c = c - \\alpha \\cdot \\frac{\\partial J}{\\partial c}\n",
    "\\]\n",
    "\n",
    "With \\( \\alpha = 0.01 \\):\n",
    "\\[\n",
    "m = 0 - 0.01 \\cdot (-41.5) = 0 + 0.415 = 0.415\n",
    "\\]\n",
    "\\[\n",
    "c = 0 - 0.01 \\cdot (-13.5) = 0 + 0.135 = 0.135\n",
    "\\]\n",
    "\n",
    "---\n",
    "\n",
    "### Why Start With \\( m = 0, c = 0 \\)?\n",
    "At the beginning, \\( m \\) and \\( c \\) are initialized to zero because it is a common starting point. Gradient descent adjusts these values iteratively to minimize the error.\n",
    "\n",
    "Let me know if you'd like further clarifications!"
   ]
  },
  {
   "cell_type": "code",
   "execution_count": null,
   "id": "ce0212b3",
   "metadata": {},
   "outputs": [],
   "source": []
  }
 ],
 "metadata": {
  "kernelspec": {
   "display_name": "Python 3 (ipykernel)",
   "language": "python",
   "name": "python3"
  },
  "language_info": {
   "codemirror_mode": {
    "name": "ipython",
    "version": 3
   },
   "file_extension": ".py",
   "mimetype": "text/x-python",
   "name": "python",
   "nbconvert_exporter": "python",
   "pygments_lexer": "ipython3",
   "version": "3.11.5"
  }
 },
 "nbformat": 4,
 "nbformat_minor": 5
}
